Loom/Release/ToProgram.lean
@@ -90,6 +90,9 @@ def flatten : {w : Nat} → Emit.MicroVerilog.Expr w → StateM FlattenSt String
   | w, .sub a b => do
       let x ← flatten a; let y ← flatten b
       freshWire w s!"{x} - {y}" (.bin .sub x y)
+  | w, .mul a b => do
+      let x ← flatten a; let y ← flatten b
+      freshWire w s!"{x} * {y}" (.bin .mul x y)
   | w, .shl a b => do
       let x ← flatten a; let y ← flatten b
       freshWire w s!"{x} << {y}" (.bin .shl x y)
@@ -299,6 +302,9 @@ private unsafe def flattenMGo :
   | w, .sub a b => do
       let x ← flattenM a; let y ← flattenM b
       freshWireM w s!"{x} - {y}" (.bin .sub x y)
+  | w, .mul a b => do
+      let x ← flattenM a; let y ← flattenM b
+      freshWireM w s!"{x} * {y}" (.bin .mul x y)
   | w, .shl a b => do
       let x ← flattenM a; let y ← flattenM b
       freshWireM w s!"{x} << {y}" (.bin .shl x y)
